## See :
## http://lod.openlinksw.com/describe/?url=http%3A%2F%2Fsw.opencyc.org%2Fconcept%2FMx4rwL1whZwpEbGdrcN5Y29ycA&graph=http%3A%2F%2Fws.nju.edu.cn%2Fnjvr%2F
## Marketing from OpenCyc: http://sw.opencyc.org/concept/Mx4rwL1whZwpEbGdrcN5Y29ycA
## Advertising: http://sw.opencyc.org/concept/Mx4rwQr8FJwpEbGdrcN5Y29ycA

@prefix schema:  <http://schema.org/> .
@prefix cvocab:  <http://open-services.net/ns/core#> .
@prefix sioc:    <http://rdfs.org/sioc/ns#> .
@prefix oplweb:  <http://www.openlinksw.com/schemas/oplweb#> .
@prefix rdfs:    <http://www.w3.org/2000/01/rdf-schema#> .
@prefix rdf:     <http://www.w3.org/1999/02/22-rdf-syntax-ns#> .
@prefix owl:     <http://www.w3.org/2002/07/owl#> .
@prefix xsd:     <http://www.w3.org/2001/XMLSchema#> .
@prefix gr:      <http://purl.org/goodrelations/v1#> .
@prefix siocs:   <http://rdfs.org/sioc/services#> .
@prefix foaf:    <http://xmlns.com/foaf/0.1/> .
@prefix wdrs:    <http://www.w3.org/2007/05/powder-s#> .
@prefix prodont: <http://www.productontology.org/id/> .
@prefix xhv:     <http://www.w3.org/1999/xhtml/vocab#> .
@prefix skos:    <http://www.w3.org/2004/02/skos/core#> .
@prefix dcterms: <http://purl.org/dc/terms/> .
@prefix ecrm:    <http://www.openlinksw.com/ontology/ecrm#> .
@prefix oplfea:  <http://www.openlinksw.com/ontology/features#> .
@prefix oplbenefit: <http://www.openlinksw.com/ontology/benefits#> . 
@prefix oplpro:  <http://www.openlinksw.com/ontology/products#> .
@prefix oplsof:  <http://www.openlinksw.com/ontology/software#> .
@prefix oplmch:  <http://www.openlinksw.com/ontology/machines#> .
@prefix opllic:  <http://www.openlinksw.com/ontology/licenses#> .
@prefix opl:     <http://www.openlinksw.com/schema/attribution#> .
@prefix cc:      <http://creativecommons.org/ns#> .
@prefix schema:  <http://schema.org/> .
@prefix oplmark:   <http://www.openlinksw.com/ontology/market#> .
@prefix oplstocks: <http://www.openlinksw.com/schemas/stocks#> .
@prefix dbpedia: <http://dbpedia.org/resource/> .

<http://www.openlinksw.com/ontology/market#> a owl:Ontology ;
  rdfs:label """OpenLink Market Segment Ontology"""^^xsd:string ;
  rdfs:comment """Ontology that defines entity and relation types used to describe entities, entity types, and relationship types
  that aid human and machine comprehensible descriptions of market segments.
  Examples include segments, seller and buyer entities etc."""@en ;
  wdrs:describedby <http://www.openlinksw.com/ontology/market> ;
  schema:creator <http://www.openlinksw.com/#this> ;
  dcterms:created "2014-08-18T13:00:00-05:00"^^xsd:dateTime ;
  dcterms:modified "2019-03-21T18:38:00-05:00"^^xsd:dateTime ;
  owl:versionInfo "1.0.0"^^xsd:string  ;
  owl:imports <http://purl.org/goodrelations/v1>  ,
              <http://xmlns.com/foaf/0.1/> ,
              <http://www.openlinksw.com/ontology/licenses#> ,
              <http://www.w3.org/2002/07/owl#> ,
              <http://www.w3.org/1999/02/22-rdf-syntax-ns#> ,
              <http://purl.org/dc/terms/> ,
              <http://www.openlinksw.com/ontology/ecrm#>  ;
  rdfs:label "OpenLink Market Segment Ontology" ;
  <http://open.vocab.org/terms/defines>
       oplmark:MarketSegment,
       <http://sw.opencyc.org/concept/Mx4rvVi84ZwpEbGdrcN5Y29ycA>,
	 	   oplmark:MarketSellerEntity,
	 	   oplmark:MarketBuyerEntity,
	 	   oplmark:seller ,
	 	   oplmark:buyer ,
	 	   oplmark:needs,
	 	   oplmark:wants,
	 	   oplmark:owns,
	 	   oplmark:hasMarketSegmentFocus,
		   oplmark:marketSize,
		   oplmark:marketSizeValue,
		   oplmark:marketSizeValueCurrencyCode,
		   oplmark:marketSizeValueScale,
		   oplmark:MarketSizeSpecification,
		   oplmark:IndustrySector,
		   oplmark:industrySegmentFocus,
		   oplmark:IndustryProductionEntity ,
		   oplmark:hasMarketCapCurrencyCode ,
		   oplmark:hasGrowthRate,
           oplmark:hasMarketCapValueScale ;
     schema:about
       	   oplmark:MarketSegment,
       	   <http://sw.opencyc.org/concept/Mx4rvVi84ZwpEbGdrcN5Y29ycA>,
	 	   oplmark:MarketSellerEntity,
	 	   oplmark:MarketBuyerEntity,
	 	   oplmark:seller ,
	 	   oplmark:buyer ,
	 	   oplmark:needs,
	 	   oplmark:wants,
	 	   oplmark:owns,
	 	   oplmark:hasMarketSegmentFocus,
		   oplmark:marketSize,
		   oplmark:marketSizeValue,
		   oplmark:marketSizeValueCurrencyCode,
		   oplmark:marketSizeValueScale,
		   oplmark:MarketSizeSpecification,
		   oplmark:IndustrySector,
		   oplmark:industrySegmentFocus,
		   oplmark:IndustryProductionEntity ,
		   oplmark:hasGrowthRate,
		   oplmark:hasMarketCapCurrencyCode ,
       oplmark:hasMarketCapValueScale .

<http://open.vocab.org/terms/defines> owl:inverseOf <http://www.w3.org/2007/05/powder-s#describedby> .

<http://www.openlinksw.com/DAV/data/turtle/market.ttl>
  a foaf:Document , schema:TechArticle ;
  rdfs:label """OpenLink Market Segment Ontology Description Document (Turtle)"""^^xsd:string ;
  cc:license <http://creativecommons.org/licenses/by-sa/3.0/> ;
  dcterms:license <http://creativecommons.org/licenses/by-sa/3.0/> ;
  schema:creator <http://www.openlinksw.com/#this> ;
  rdfs:comment """This is a turtle document that uses Linked Data oriented content to describe an OpenLink ontology for Market Segment."""@en ;
  foaf:primaryTopic <http://www.openlinksw.com/ontology/market#> ;
  dcterms:created "2014-05-18T13:00:00-05:00"^^xsd:dateTime ;
  dcterms:modified "2019-03-21T18:38:00-05:00"^^xsd:dateTime ;
  xhv:canonical <http://www.openlinksw.com/ontology/market> ;
  xhv:describes <http://www.openlinksw.com/ontology/market#> ;
  schema:about <http://www.openlinksw.com/ontology/market#> ;
  dcterms:subject <http://www.openlinksw.com/ontology/market#> .

<http://www.openlinksw.com/data/turtle/market.ttl>
   a foaf:Document,
     schema:WebPage;
   rdfs:label """OpenLink Market Segment Ontology Description Document (Turtle)"""^^xsd:string ;
   rdfs:comment """Entity & Relaitonship Types that aid the process of
				describing a market segment in a form that's
				comprehensible to both humans and machines.
				"""@en ;
   schema:creator <http://kingsley.idehen.net/dataspace/person/kidehen#this> ;
   dcterms:created "2014-08-18T13:00:00-05:00"^^xsd:dateTime ;
   dcterms:modified "2019-03-21T18:38:00-05:00"^^xsd:dateTime ;
   cc:license <http://creativecommons.org/licenses/by/4.0/deed.en_US> ;
   cc:attributionName "OpenLink Software" ;
   cc:attributionURL <http://www.openlinksw.com/dataspace/organization/openlink#this> ;
   foaf:primaryTopic <http://www.openlinksw.com/ontology/market#> ;
   xhv:canonical <http://www.openlinksw.com/ontology/market> ;
   xhv:describes <http://www.openlinksw.com/ontology/market#> ;
   schema:about <http://www.openlinksw.com/ontology/market#> ;
   dcterms:subject <http://www.openlinksw.com/ontology/market#> .

<http://www.openlinksw.com/ontology/market>
  a foaf:Document , schema:TechArticle ;
  rdfs:label """OpenLink Market Segment Ontology Description Document"""^^xsd:string ;
  cc:license <http://creativecommons.org/licenses/by-sa/3.0/> ;
  dcterms:created "2014-05-18T13:00:00-05:00"^^xsd:dateTime ;
  dcterms:modified "2019-03-21T18:38:00-05:00"^^xsd:dateTime ;
  schema:creator <http://www.openlinksw.com/#this> ;
  rdfs:comment """This is a document that uses Linked Data oriented content to describe OpenLink Market Segment Ontology."""@en ;
  dcterms:subject <http://www.openlinksw.com/ontology/market#> ;
  foaf:primaryTopic <http://www.openlinksw.com/ontology/market#> ;
  foaf:topic
       oplmark:MarketSegment,
       <http://sw.opencyc.org/concept/Mx4rvVi84ZwpEbGdrcN5Y29ycA>,
	 	   oplmark:MarketSellerEntity,
	 	   oplmark:MarketBuyerEntity,
	 	   oplmark:seller ,
	 	   oplmark:buyer ,
	 	   oplmark:needs,
	 	   oplmark:wants,
	 	   oplmark:hasMarketSegmentFocus,
		   oplmark:marketSize,
		   oplmark:marketSizeValue,
		   oplmark:marketSizeValueCurrencyCode,
		   oplmark:marketSizeValueScale,
		   oplmark:MarketSizeSpecification,
		   oplmark:IndustrySector,
		   oplmark:industrySegmentFocus,
		   oplmark:IndustryProductionEntity ,
		   oplmark:hasMarketCapCurrencyCode ,
		   oplmark:hasGrowthRate,
       oplmark:hasMarketCapValueScale .


# <-------------- Market Classes --------------> #

oplmark:IndustrySector  a owl:Class  ;
  owl:equivalentClass <http://sw.opencyc.org/concept/Mx4rvxQhVpwpEbGdrcN5Y29ycA> ;
  rdfs:label "IndustrySector" ;
  skos:altLabel "Industry Sector" ;
  schema:name "Industry Sector" ;
  rdfs:comment """Classifier for goods and services production focus."""@en .

oplmark:MarketSegment a owl:Class ;
  owl:equivalentClass <http://sw.opencyc.org/concept/Mx4rvVi84ZwpEbGdrcN5Y29ycA> ;
  rdfs:label "MarketSegment" ;
  skos:altLabel "Market Segment" ;
  schema:name "Market Segment" ;
  rdfs:comment """A market segment."""@en ;
  rdfs:isDefinedBy <http://www.openlinksw.com/ontology/market#>  .

  oplmark:MarketSegmentIaaS rdfs:subClassOf oplmark:MarketSegment ;
    rdfs:label "Infrastructure as-a-Service (IaaS)" ;
    skos:altLabel "IaaS" ;
    schema:name "Infrastructure as-a-Service (IaaS)" ;
	schema:image <https://s3.amazonaws.com/ceblog/wp-content/uploads/2018/06/20124711/saas-conversion-funnel-15.png>,
	 			 <http://cloudonmove.com/wp-content/uploads/2017/07/Cloud-service-models-e1500291137271.png> ;
    rdfs:comment """Critical computing infrastructure deployed to the cloud 
  				for exploitation by on- and off-premise software projects and solutions.
  			 """@en ;
    skos:related dbpedia:Platform_as_a_service, dbpedia:Software_as_a_service, dbpedia:Cloud_computing ;
    rdfs:isDefinedBy <http://www.openlinksw.com/ontology/market#>  .
	
oplmark:MarketSegmentPaaS rdfs:subClassOf oplmark:MarketSegment ;
  rdfs:label "Infrastructure as-a-Service (PaaS)" ;
  skos:altLabel "PaaS" ;
  schema:name "Platform as-a-Service (PaaS)" ;
  schema:image <http://cloudonmove.com/wp-content/uploads/2017/07/Cloud-service-models-e1500291137271.png> ;
  rdfs:comment """Application Development Services packaged as a suite and deployed to the cloud 
				  for exploitation by on- and off-premise software projects and solutions.
			 """@en ;
  skos:related dbpedia:Platform_as_a_service, dbpedia:Software_as_a_service, dbpedia:Cloud_computing ;
  rdfs:isDefinedBy <http://www.openlinksw.com/ontology/market#>  .
	
  oplmark:MarketSegmentSaaS rdfs:subClassOf oplmark:MarketSegment ;
    rdfs:label "Software as-a-Service (SaaS)" ;
    skos:altLabel "SaaS" ;
    schema:name "Software as-a-Service (SaaS)" ;
	schema:image <https://s3.amazonaws.com/ceblog/wp-content/uploads/2018/06/20124711/saas-conversion-funnel-15.png> ;
    rdfs:comment """Category of Application Software (e.g., CRM, HR, ERP etc.) deployed to the cloud 
  				for exploitation by on- and off-premise software projects and solutions.
  			 """@en ;
    skos:related dbpedia:Software_as_a_service, dbpedia:Cloud_computing ;
    rdfs:isDefinedBy <http://www.openlinksw.com/ontology/market#>  .
	 
  oplmark:MarketSegmentIPaaS rdfs:subClassOf oplmark:MarketSegment ;
    rdfs:label "Integration Platform as-a-Service (IPaaS)" ;
    skos:altLabel "IPaaS" ;
    schema:name "Integration Platform as-a-Service (IPaaS)" ;
	schema:image <https://boomi.com/wp-content/uploads/2016/12/Boomi-iPaaS-schematic.png> ;
    rdfs:comment """Category of software functioning as a Middleware Suite covering 
					services, applications, and data integration deployed to the cloud 
					for exploitation by on- and off-premise software projects and solutions.
				 """@en ;
	skos:related <https://www.gartner.com/it-glossary/information-platform-as-a-service-ipaas/#class>, 
				dbpedia:Cloud_computing ;
    rdfs:isDefinedBy <http://www.openlinksw.com/ontology/market#>  .

oplmark:MarketSegmentDaaS rdfs:subClassOf oplmark:MarketSegment ;
  rdfs:label "Data as-a-Service (DaaS)" ;
  skos:altLabel "DaaS" ;
  schema:name "Data as-a-Service (DaaS)" ;
  schema:image <http://www.corporate360.us/images/1uy.jpg> ;
  rdfs:comment """Category of software functioning as a Data Space Collective deployed to the cloud 
				for exploitation by on- and off-premise software projects and solutions.
			 """@en ;
  skos:related dbpedia:Data_as_a_service, dbpedia:Cloud_computing ;
  rdfs:isDefinedBy <http://www.openlinksw.com/ontology/market#>  .
  
  oplmark:MarketSegmentDBaaS rdfs:subClassOf oplmark:MarketSegment ;
    rdfs:label "Database as-a-Service (DBaaS)" ;
    skos:altLabel "DBaaS" ;
    schema:name "Database as-a-Service (DaaS)" ;
	schema:image <https://www.researchgate.net/profile/Luis_Bastiao_Silva/publication/260374716/figure/fig5/AS:613853259919385@1523365430811/Database-as-a-Service.png> ;
    rdfs:comment """Category of software functioning as a Database Management System (DBMS) deployed to the cloud 
					for exploitation by on- and off-premise software projects and solutions.
				 """@en ;
	skos:related dbpedia:Data_as_a_service, dbpedia:Cloud_database, dbpedia:Cloud_computing ;
    rdfs:isDefinedBy <http://www.openlinksw.com/ontology/market#>  .

<http://sw.opencyc.org/concept/Mx4rvVi84ZwpEbGdrcN5Y29ycA> a owl:Class ;
  rdfs:label "Market Category" ;
  schema:name "Market Category" ;
  rdfs:comment """OpenCyc market categorization class."""@en .

oplmark:IndustryProductionEntity a owl:Class ;
  rdfs:label "IndustryProductionEntity" ;
  skos:altLabel "Industry Production" ;
  schema:name "Industry Production Entity" ;
  rdfs:comment """Producer of goods and services targeting a specific industry sector."""@en ;
  rdfs:subClassOf gr:BusinessEntity;
  rdfs:isDefinedBy <http://www.openlinksw.com/ontology/market#>  .

oplmark:MarketSellerEntity a owl:Class ;
  rdfs:label "MarketSellerEntity" ;
  skos:altLabel "Market Seller" ;
  schema:name "Market Seller Entity" ;
  rdfs:comment """Organization or Person that sells products/services targeting a specific market"""@en ;
  rdfs:subClassOf gr:BusinessEntity;
  rdfs:isDefinedBy <http://www.openlinksw.com/ontology/market#>  .

oplmark:MarketBuyerEntity a owl:Class ;
  rdfs:label "MarketSellerEntity" ;
  schema:name "Market Buyer Entity" ;
  skos:altLabel "Market Buyer Entity" ;
  rdfs:comment """Organization or Person that seeks, wants, or needs products/services targeting a specific market"""@en ;
  rdfs:subClassOf gr:BusinessEntity ;
  rdfs:isDefinedBy <http://www.openlinksw.com/ontology/market#>  .

oplmark:MarketSizeSpecification a owl:Class ;
  rdfs:label "MarketSizeSpecification" ;
  skos:altLabel "Market Size" ;
  schema:name "Market Size Specification" ;
  owl:equivalentClass <https://twitter.com/hashtag/MarketSizeSpecification#this> ;
  rdfs:isDefinedBy <http://www.openlinksw.com/ontology/market#>  .

<https://twitter.com/hashtag/MarketSizeSpecification#this> a owl:Class ;
  rdfs:label "MarketSizeSpecification" ;
  schema:name "MarketSizeSpecification" ;
  rdfs:comment """Twitter Market Size Specification. This class was defined
  via a Tweet, using Nanotation."""@en ;
  wdrs:describedby <> .


# <-------------- Market Properties --------------> #

oplmark:needs a rdf:Property, owl:ObjectProperty ;
  rdfs:label "needs" ;
  schema:name "needs" ;
  skos:altLabel "needs" ;
  rdfs:comment """Relationship property that associates an Agent with something it needs, but doesn't necessarily want,
                  and isn't necessarily seeking. Hence the super property relation in regards to schema:seeks."""@en ;
  schema:domainIncludes schema:Organization,
                        ecrm:Company,
                        foaf:Organization,
                        schema:Person,
                        foaf:Person,
                        oplmark:MarketBuyerEntity,
                        gr:BusinessEntity ;
  rdfs:domain oplmark:MarketBuyerEntity ;
  rdfs:range oplbenefit:Benefit ;
  rdfs:subPropertyOf schema:seeks ;
  rdfs:isDefinedBy <http://www.openlinksw.com/ontology/market#>  .

oplmark:wants a rdf:Property, owl:ObjectProperty ;
  rdfs:label "wants" ;
  schema:name "wants" ;
  skos:altLabel "wants" ;
  rdfs:comment """Relationship property that associates an Agent with something it wants, but doesn't necessarily need,
                  and isn't necessarily seeking. Hence the super property relation in regards to schema:seeks."""@en ;
  rdfs:domain oplmark:MarketBuyerEntity ;
  rdfs:range oplbenefit:Benefit ;
  rdfs:subPropertyOf schema:seeks ;
  rdfs:isDefinedBy <http://www.openlinksw.com/ontology/market#>  .

oplmark:owns a rdf:Property, owl:ObjectProperty, owl:TransitiveProperty ;
  rdfs:subPropertyOf gr:owns;
  rdfs:label "owns" ;
  schema:name "owns" ;
  skos:altLabel "owns" ;
  rdfs:comment """The subject of this relationship type possesses verifiable ownership rights over the relationship subject. Naturally, this kind of relationship type is transitive."""@en ;
  rdfs:domain foaf:Agent ;
  rdfs:range owl:Thing ;
  rdfs:isDefinedBy <http://www.openlinksw.com/ontology/market#>  .

oplmark:hasMarketSegmentFocus a rdf:Property, owl:ObjectProperty ;
  rdfs:label "hasMarketSegmentFocus" ;
  skos:altLabel "market segment focus" ;
  schema:name "Market Segment Focus" ;
  rdfs:comment """Focal point of a specific segment (part) of a market."""@en ;
  rdfs:domain oplmark:MarketSellerEntity,
              oplmark:MarketBuyerEntity ;
  schema:domainIncludes
              schema:Product,
              gr:BusinessEntity ;
  rdfs:range oplmark:MarketSegment ;
  owl:equivalentProperty <https://twitter.com/hashtag/marketFocus#this> ;
  rdfs:isDefinedBy <http://www.openlinksw.com/ontology/market#>  .

schema:Product owl:disjointWith gr:BusinessEntity .

<https://twitter.com/hashtag/marketFocus#this> a rdf:Property ;
  rdfs:label "marketFocus" ;
  schema:name "Market Focus" ;
  rdfs:comment """Relation for associating various entity types with a market segment of focus. This relation was defined
  via a Tweet, using Nanotation."""@en ;
  wdrs:describedby <> .

oplmark:marketSize a rdf:Property, owl:ObjectProperty ;
  rdfs:label "marketSize" ;
  skos:altLabel "market segment size" ;
  schema:name "Market Segment Size" ;
  rdfs:domain
     <http://sw.opencyc.org/concept/Mx4rvVi84ZwpEbGdrcN5Y29ycA>,
     oplmark:MarketSegment ;
  rdfs:range  oplmark:MarketSizeSpecification ;
  owl:equivalentProperty <https://twitter.com/hashtag/marketSize#this> ;
  rdfs:isDefinedBy <http://www.openlinksw.com/ontology/market#>  .

<https://twitter.com/hashtag/marketSize#this>  a rdf:Property ;
  rdfs:label "marketSize" ;
  schema:name "Market Size" ;
  rdfs:comment """Relation for associating various entity types with a market segment of size. This relation was defined
  via a Tweet, using Nanotation."""@en ;
  wdrs:describedby <> .


oplmark:marketSizeValue a rdf:Property, owl:ObjectProperty ;
  rdfs:label "marketSizeValue" ;
  skos:altLabel "market size value" ;
  schema:name "Market Size value" ;
  rdfs:comment """Market Size Numeric Value"""@en ;
  rdfs:domain oplmark:MarketSizeSpecification  ;
  rdfs:range xsd:decimal ;
  rdfs:isDefinedBy <http://www.openlinksw.com/ontology/market#>  .

oplmark:marketSizeValueCurrencyCode a rdf:Property, owl:ObjectProperty ;
  rdfs:label "marketSizeValueCurrencyCode" ;
  skos:altLabel "market size value currency code" ;
  schema:name "Market Size value currency code" ;
  rdfs:comment """Market Size Numeric Value Currency Code e.g., USD."""@en ;
  rdfs:domain oplmark:MarketSizeSpecification  ;
  rdfs:range xsd:string ;
  rdfs:isDefinedBy <http://www.openlinksw.com/ontology/market#>  .

oplmark:marketSizeValueScale a rdf:Property, owl:ObjectProperty ;
  rdfs:label "marketSizeValueScale" ;
  skos:altLabel "market size value scale" ;
  schema:name "Market Size value scale" ;
  rdfs:comment """Market Size Numeric Value Scale e.g., Million, Billion, Trillion."""@en ;
  rdfs:domain oplmark:MarketSizeSpecification  ;
  rdfs:range xsd:string ;
  rdfs:isDefinedBy <http://www.openlinksw.com/ontology/market#>  .

oplmark:industrySegmentFocus a rdfs:Property, owl:ObjectProperty ;
  rdfs:label "industrySegmentFocus" ;
  skos:altLabel "industry segment focus" ;
  schema:name "Industry Segment Focus" ;
  rdfs:comment """Relationship property (predicate) that associates an producer of goods and services with an industry sector"""@en ;
  rdfs:range oplmark:IndustrySector ;
  rdfs:domain oplmark:IndustryProductionEntity .

oplmark:seller a rdf:Property, owl:ObjectProperty ;
  rdfs:label "seller" ;
  skos:altLabel "seller" ;
  schema:name "seller" ;
  rdfs:comment """Market Seller"""@en ;
  rdfs:domain oplmark:MarketSegment  ;
  rdfs:range oplmark:MarketSellerEntity ;
  rdfs:isDefinedBy <http://www.openlinksw.com/ontology/market#>  .

oplmark:buyer a rdf:Property, owl:ObjectProperty ;
  rdfs:label "buyer" ;
  skos:altLabel "buyer" ;
  schema:name "buyer" ;
  rdfs:comment """Market Buyer"""@en ;
  rdfs:domain oplmark:MarketSegment  ;
  rdfs:range oplmark:MarketBuyerEntity ;
  rdfs:isDefinedBy <http://www.openlinksw.com/ontology/market#>  .

oplmark:hasMarketCapCurrencyCode
   a rdf:Property, owl:DatatypeProperty ;
   rdfs:label "hasMarketCapCurrencyCode" ;
   skos:altLabel "market cap currency code" ;
   schema:name "Market Cap Currency code" ;
   rdfs:isDefinedBy <http://www.openlinksw.com/schemas/stocks#> ;
   rdfs:comment """Associates a Market Capitalization Specification with a currency code"""@en ;
   rdfs:domain oplstocks:MarketCapSpecification ;
   rdfs:range xsd:decimal .

oplmark:hasGrowthRate
  a rdf:Property, owl:DatatypeProperty ;
  rdfs:label "hasGrowthRate" ;
  skos:altLabel "CAGR" ;
  schema:name "Compound Annual Growth Rate" ;
  rdfs:isDefinedBy <http://www.openlinksw.com/ontology/market#>  ;
  rdfs:comment """Estimated Annual Growth Rate"""@en ;
  rdfs:domain oplmark:MarketSizeSpecification  ;
  rdfs:range xsd:decimal .
	  
oplmark:hasMarketCapValueScale
   a rdf:Property, owl:DatatypeProperty;
   rdfs:label "hasMarketCapValueScale";
   skos:altLabel "market cap value scale" ;
   schema:name "Market Cap value scale" ;
   rdfs:isDefinedBy <http://www.openlinksw.com/schemas/stocks#> ;
   rdfs:comment """Associates a Market Capitalization Specification with a value scale e.g., Millions, Billions etc."""@en ;
   rdfs:domain oplstocks:MarketCapSpecification ;
   rdfs:range xsd:decimal .

