@prefix schema:  <http://schema.org/> .
@prefix dbpedia: <http://dbpedia.org/resource/> .
@prefix cvocab:  <http://open-services.net/ns/core#> .
@prefix sioc:    <http://rdfs.org/sioc/ns#> .
@prefix oplweb:  <http://www.openlinksw.com/schemas/oplweb#> .
@prefix rdfs:    <http://www.w3.org/2000/01/rdf-schema#> .
@prefix rdf:     <http://www.w3.org/1999/02/22-rdf-syntax-ns#> .
@prefix owl:     <http://www.w3.org/2002/07/owl#> .
@prefix xsd:     <http://www.w3.org/2001/XMLSchema#> .
@prefix gr:      <http://purl.org/goodrelations/v1#> .
@prefix siocs:   <http://rdfs.org/sioc/services#> .
@prefix foaf:    <http://xmlns.com/foaf/0.1/> .
@prefix wdrs:    <http://www.w3.org/2007/05/powder-s#> .
@prefix prodont: <http://www.productontology.org/id/> .
@prefix xhv:     <http://www.w3.org/1999/xhtml/vocab#> .
@prefix skos:    <http://www.w3.org/2004/02/skos/core#> .
@prefix dcterms: <http://purl.org/dc/terms/> .
@prefix odbc:    <http://www.openlinksw.com/ontology/odbc#> .
@prefix oplpro:  <http://www.openlinksw.com/ontology/products#> .
@prefix oplsof:  <http://www.openlinksw.com/ontology/software#> .
@prefix opllic:  <http://www.openlinksw.com/ontology/licenses#> .
@prefix oplben:  <http://www.openlinksw.com/ontology/benefits#> .
@prefix opl:     <http://www.openlinksw.com/schema/attribution#> .
@prefix cc:      <http://creativecommons.org/ns#> .

<http://www.openlinksw.com/dataspace/organization/openlink#this>
   a <http://www.w3.org/ns/org#Organization> , schema:Organization;
   rdfs:label "OpenLink Software" ;
   schema:name "OpenLink Software" ;
   schema:logo <http://www.openlinksw.com/images/openlink150.gif> ;
   foaf:logo <http://www.openlinksw.com/images/openlink150.gif> ;
   dcterms:description """OpenLink Software is a privately held company founded in 1992 by its President & CEO, Kingsley
   Idehen. The company is an industry acclaimed technology innovator in the following areas: ODBC, ODBC, ADO.NET, and OLE-DB
   compliant Data Access Drivers for Oracle,SQL Server, DB2, Informix, Ingres, Sybase, Progress, MySQL, and PostgreSQL;
   Object-Relational Database Technology; Data Integration Middleware (Virtual Database Engine Technology); Hybrid Data Servers
   for SQL, XML, RDF, and Full Text data sources; Web Application Server Technology Application Integration Middleware (Web
   Services Platforms and Service Oriented Architecture); Business Process Management & Integration; Distributed Collaborative
   Applications Platforms (Weblogs, Wikis, Feed Aggregation and Syndication, Web File Systems, Discussion Forums etc.)"""@en ;
   rdfs:comment """OpenLink Software is an acclaimed technology innovator and leading vendor of industry
   standards compliant data access, integration, and management technology. """@en ;
   schema:email "sales@openlinksw.com";
   schema:about <http://www.openlinksw.com/dataspace/organization/openlink#this> ;
   schema:url <http://www.openlinksw.com/> ;
   schema:addressLocality "Burlington" ;
   schema:postOfficeBoxNumber "Suite 265" ;
   schema:addressCountry "US" ;
   schema:postalCode "MA-01803" ;
   schema:streetAddress "10 Burlington Mall Road" ;
   schema:telephone "+1 781 273 0900" ;
   schema:faxNumber "+1 781 229 8030" .


<http://www.openlinksw.com/ontology/odbc#> a owl:Ontology ;
  rdfs:label """OpenLink ODBC Driver Ontology of Terms"""^^xsd:string ;
  dcterms:title """OpenLink ODBC Driver Ontology of Terms"""^^xsd:string ;
  rdfs:comment """Ontology that defines entity and relation types used to describe odbc drivers. Examples include
  connectivity methods, various application programs etc. """@en ;
  wdrs:describedby <http://www.openlinksw.com/ontology/odbc> ;
  dcterms:created "2019-04-24T11:00:00-05:00"^^xsd:dateTime ;
  dcterms:modified "2019-04-24T11:00:00-05:00"^^xsd:dateTime ;
  foaf:depiction <https://s-media-cache-ak0.pinimg.com/originals/ef/b2/7e/efb27e54ef098c18a93aa8a074d5817d.jpg> ;
  schema:creator <http://www.openlinksw.com/#this> ;
  owl:versionInfo "1.0.0"^^xsd:string ;
  <http://open.vocab.org/terms/defines>
      odbc:OpenDatabaseConnectivityDriver ,
      odbc:DBVendorNativeNetworkConnectivity,
      odbc:DBVendorProvidedNetworkConnectivity,
      odbc:DBVendorIndependentNetworkConnectivity,
      odbc:isOpsysArchitectureCompliant,
      odbc:isUsableWith,
      odbc:hasOSAvailability,
      odbc:hasDBMSReleaseSupport,
      odbc:isODBCLevelCompliant,
      odbc:hasScrollableCursorTypeSupport,
      odbc:hasDistributedTransactionMonitorSupport,
      odbc:hasMultipleActiveStatementsSupport ,
      odbc:hasDataTransmissionEncryptionSupport,
      odbc:hasFineGrainedAccessControls,
      odbc:hasDatabaseNetworkConnectivityMethod,
      odbc:hasProtocolSupport ,
      odbc:StaticScrollableCursor ,
      odbc:ScrollableCursor ,
      odbc:DistributedTransactionMonitor ,
      odbc:DynamicScrollableCursor ,
      odbc:KeySetScrollableCursor ,
      odbc:MixedScrollableCursor ,
      odbc:isChangeSenstive ,
      odbc:hasCursorSupport ,
      odbc:isFullyChangeSenstive ,
      odbc:isKeySetDriven ,
      odbc:isDynamicKeySetDriven ,
      odbc:hasConnectionPoolingSupport ,
      odbc:hasRealApplicationClustorSupport ,
      odbc:hasMultipleActiveStatementsSupport ;
   schema:about
      odbc:OpenDatabaseConnectivityDriver ,
      odbc:DBVendorNativeNetworkConnectivity,
      odbc:DBVendorProvidedNetworkConnectivity,
      odbc:DBVendorIndependentNetworkConnectivity,
      odbc:isOpsysArchitectureCompliant,
      odbc:isUsableWith,
      odbc:hasOSAvailability,
      odbc:hasDBMSReleaseSupport,
      odbc:isODBCLevelCompliant,
      odbc:hasScrollableCursorTypeSupport,
      odbc:hasDistributedTransactionMonitorSupport,
      odbc:hasDataTransmissionEncryptionSupport,
      odbc:hasMultipleActiveStatementsSupport ,
      odbc:hasFineGrainedAccessControls,
      odbc:hasDatabaseNetworkConnectivityMethod,
      odbc:hasProtocolSupport ,
      odbc:StaticScrollableCursor ,
      odbc:ScrollableCursor ,
      odbc:DistributedTransactionMonitor ,
      odbc:DynamicScrollableCursor ,
      odbc:KeySetScrollableCursor ,
      odbc:MixedScrollableCursor ,
      odbc:isChangeSenstive ,
      odbc:hasCursorSupport ,
      odbc:isFullyChangeSenstive ,
      odbc:isKeySetDriven ,
      odbc:isDynamicKeySetDriven ,
      odbc:hasConnectionPoolingSupport ,
      odbc:hasRealApplicationClustorSupport ,
      odbc:hasMultipleActiveStatementsSupport .

<http://open.vocab.org/terms/defines> owl:inverseOf <http://www.w3.org/2007/05/powder-s#describedby> .

<http://www.openlinksw.com/DAV/data/turtle/odbc.ttl>
  a foaf:Document , schema:TechArticle ;
  rdfs:label """OpenLink ODBC Driver Ontology Description Document (Turtle)"""^^xsd:string ;
  cc:license <http://creativecommons.org/licenses/by-sa/3.0/> ;
  schema:creator <http://www.openlinksw.com/#this> ;
  rdfs:comment """This is a turtle document that uses Linked Data oriented content to describe an OpenLink ontology for ODBC Driver. """@en ;
  foaf:primaryTopic <http://www.openlinksw.com/ontology/odbc#> ;
  dcterms:created "2019-04-24T13:00:00-05:00"^^xsd:dateTime ;
  dcterms:modified "2019-04-24T13:38:00-05:00"^^xsd:dateTime ;
  xhv:canonical <http://www.openlinksw.com/ontology/odbc> ;
  xhv:describes <http://www.openlinksw.com/ontology/odbc#> ;
  schema:about <http://www.openlinksw.com/ontology/odbc#> ;
  dcterms:subject <http://www.openlinksw.com/ontology/odbc#> .

<http://www.openlinksw.com/data/turtle/odbc.ttl>
  a foaf:Document , schema:TechArticle ;
  rdfs:label """OpenLink ODBC Driver Ontology Description Document (Turtle)"""^^xsd:string ;
  cc:license <http://creativecommons.org/licenses/by-sa/3.0/> ;
  dcterms:created "2019-04-24T13:00:00-05:00"^^xsd:dateTime ;
  dcterms:modified "2019-04-24T13:38:00-05:00"^^xsd:dateTime ;
  schema:creator <http://www.openlinksw.com/#this> ;
  rdfs:comment """This is a turtle document that uses Linked Data oriented content to describe OpenLink ODBC Driver Ontology. """@en ;
  foaf:primaryTopic <http://www.openlinksw.com/ontology/odbc#> ;
  xhv:canonical <http://www.openlinksw.com/ontology/odbc> ;
  xhv:describes <http://www.openlinksw.com/ontology/odbc#> ;
  schema:about <http://www.openlinksw.com/ontology/odbc#> ;
  dcterms:subject <http://www.openlinksw.com/ontology/odbc#> .

<http://www.openlinksw.com/ontology/odbc>
  a foaf:Document , schema:TechArticle ;
  rdfs:label """OpenLink ODBC Driver Ontology Description Document"""^^xsd:string ;
  cc:license <http://creativecommons.org/licenses/by-sa/3.0/> ;
  dcterms:created "2019-04-24T13:00:00-05:00"^^xsd:dateTime ;
  dcterms:modified "2019-04-24T13:38:00-05:00"^^xsd:dateTime ;
  schema:creator <http://www.openlinksw.com/#this> ;
  rdfs:comment """This is a document that uses Linked Data oriented content to describe OpenLink ODBC Driver Ontology. """@en ;
  dcterms:subject <http://www.openlinksw.com/ontology/odbc#> ;
  foaf:primaryTopic <http://www.openlinksw.com/ontology/odbc#> ;
  foaf:topic
      odbc:OpenDatabaseConnectivityDriver ,
      odbc:DBVendorNativeNetworkConnectivity,
      odbc:DBVendorProvidedNetworkConnectivity,
      odbc:DBVendorIndependentNetworkConnectivity,
      odbc:isOpsysArchitectureCompliant,
      odbc:isUsableWith,
      odbc:hasOSAvailability,
      odbc:hasDBMSReleaseSupport,
      odbc:isODBCLevelCompliant,
      odbc:hasScrollableCursorTypeSupport,
      odbc:hasMultipleActiveStatementsSupport ,
      odbc:hasDistributedTransactionMonitorSupport,
      odbc:hasDataTransmissionEncryptionSupport,
      odbc:hasFineGrainedAccessControls,
      odbc:hasDatabaseNetworkConnectivityMethod,
      odbc:hasProtocolSupport ,
      odbc:StaticScrollableCursor ,
      odbc:ScrollableCursor ,
      odbc:DistributedTransactionMonitor ,
      odbc:DynamicScrollableCursor ,
      odbc:KeySetScrollableCursor ,
      odbc:MixedScrollableCursor ,
      odbc:isChangeSenstive ,
      odbc:hasCursorSupport ,
      odbc:isFullyChangeSenstive ,
      odbc:isKeySetDriven ,
      odbc:isDynamicKeySetDriven ,
      odbc:hasConnectionPoolingSupport ,
      odbc:hasRealApplicationClustorSupport ,
      odbc:hasMultipleActiveStatementsSupport .

# <-------------- ODBC Ontology --------------> #

# <-------------- ODBC Ontology Classes --------------> #

odbc:DistributedTransactionMonitor a owl:Class ;
   rdfs:label "Distributed Transaction Monitor"@en ;
   rdfs:comment """Technology for managing Atomicity, Consistency, Isolation, and Durability of transactions across machine boundaries, on a distributed network. """@en ;
   skos:altLabel "ODBC Driver"@en  ;
   rdfs:isDefinedBy <http://www.openlinksw.com/ontology/odbc#> .

odbc:ScrollableCursor a owl:Class ;
   rdfs:label "Scrollable Cursor"@en ;
   rdfs:comment """Data paging and scrolling [sliding window] mechanism with varying levels of change sensitivity in regards to query resultset [solution] row membership, order, and values. """@en ;
   skos:altLabel "ODBC Driver"@en  ;
   rdfs:isDefinedBy <http://www.openlinksw.com/ontology/odbc#> .

odbc:StaticScrollableCursor a owl:Class ;
   rdfs:subClassOf odbc:ScrollableCursor ;
   rdfs:label "Static Scrollable Cursor"@en ;
   rdfs:comment """	Data paging and scrolling [sliding window] mechanism that's insensitive to changes (membership, order, and values) that occur to a query resultset (solution) after it has been created. """@en ;
   skos:altLabel "ODBC Driver"@en  ;
   rdfs:isDefinedBy <http://www.openlinksw.com/ontology/odbc#> .

odbc:DynamicScrollableCursor a owl:Class ;
  rdfs:subClassOf odbc:ScrollableCursor ;
  rdfs:label "Dynamic Scrollable Cursor"@en ;
  rdfs:comment """Data paging and scrolling [sliding window]mechanism that's sensitive to changes (membership, order, and values) that occur
					to a query resultset (solution) after it has been created. This behaviour is achieved by creating
					keysets afresh [from tables used to drive a query resultset or solution] prior to each scroll (paging) operation. """@en ;
  skos:altLabel "ODBC Driver"@en  ;
  rdfs:isDefinedBy <http://www.openlinksw.com/ontology/odbc#> .

odbc:KeySetScrollableCursor a owl:Class ;
  rdfs:subClassOf odbc:ScrollableCursor ;
  rdfs:label "Keyset Driven Scrollable Cursor"@en ;
  rdfs:comment """Data paging and scrolling [sliding window] mechanism that's sensitive to row value changes while being partially sensitive to
				changes in membership and order, once opened. This behaviour is the result of keysets being created from primary keys of tables used to derive a query resultset (solution). """@en ;
  skos:altLabel "ODBC Driver"@en  ;
  rdfs:isDefinedBy <http://www.openlinksw.com/ontology/odbc#> .

odbc:MixedScrollableCursor a owl:Class ;
  rdfs:subClassOf odbc:ScrollableCursor ;
  rdfs:label "Mixed Scrollable Cursor"@en ;
  rdfs:comment """Data paging and scrolling [sliding window] mechanism that's partially sensitive to row value changes while also being partially sensitive to
				changes in membership and order, once opened. This behaviour is the result of keysets [with fixed sizes] being created
				from primary keys of tables used to derive a query resultset (solution). """@en ;
  rdfs:isDefinedBy <http://www.openlinksw.com/ontology/odbc#> .

odbc:OpenDatabaseConnectivityDriver  a owl:Class ;
   rdfs:subClassOf oplsof:ApplicationProgram, schema:SoftwareApplication ;
   rdfs:label "Open Database Connectivity Driver"@en ;
   skos:altLabel "ODBC Driver"@en  ;
   rdfs:isDefinedBy <http://www.openlinksw.com/ontology/odbc#> .

oplsof:DatabaseNetworkConnectivityMethod a owl:Class ;
   rdfs:subClassOf <http://sw.opencyc.org/concept/Mx4rvWMjUJwpEbGdrcN5Y29ycA> ;
   rdfs:label "Database Network Connectivity Method"@en ;
   rdfs:comment """How a driver connects to a DBMS over a network. """@en ;
   rdfs:isDefinedBy <http://www.openlinksw.com/ontology/odbc#> .

odbc:DBVendorNativeNetworkConnectivity a owl:Class ;
   rdfs:subClassOf <http://sw.opencyc.org/concept/Mx4rvWMjUJwpEbGdrcN5Y29ycA>, oplsof:DatabaseNetworkConnectivityMethod ;
   rdfs:label "DBVendorNativeNetworkConnectivity"@en  ;
   skos:altLabel "Database Vendor Provided Native Network Connectivity"@en ;
   rdfs:comment """In this form of DBMS connectivity, a driver leverages built-in network connectivity to a DBMS using
			a library provided by the target DBMS vendor, that's pre-installed as part of the DBMS product packaging.
			It has the advantage of providing a convenient installation and configuration experience to driver users.
			It has the disadvantage of delivering unpredictable experience and sophistication in areas such as cost-effective
			administration, privacy, security, and fine-grained access controls. """@en ;
   rdfs:isDefinedBy <http://www.openlinksw.com/ontology/odbc#> .

odbc:DBVendorProvidedNetworkConnectivity a owl:Class ;
   rdfs:subClassOf <http://sw.opencyc.org/concept/Mx4rvWMjUJwpEbGdrcN5Y29ycA>, oplsof:DatabaseNetworkConnectivityMethod ;
   rdfs:label "DBVendorProvidedNetworkConnectivity"@en  ;
   skos:altLabel "Database Vendor Provided Network Client Connectivity"@en  ;
   rdfs:comment """In this form of DBMS connectivity, a driver depends on client networking services provided the vendor of
			a DBMS targeted by a driver. It has the disadvantage of introducing preinstallation and configuration
			as driver usage prequisites. It has the advantage of providing a high-performance networking layer [in many cases]
			that's fine-tuned for its target DBMS. """@en  ;
   rdfs:isDefinedBy <http://www.openlinksw.com/ontology/odbc#> .


odbc:DBVendorIndependentNetworkConnectivity a owl:Class ;
   rdfs:subClassOf <http://sw.opencyc.org/concept/Mx4rvWMjUJwpEbGdrcN5Y29ycA>, oplsof:DatabaseNetworkConnectivityMethod ;
   rdfs:label "DBVendorIndependentNetworkConnectivity"@en  ;
   skos:altLabel "Database Vendor Independent Network Connectivity"@en  ;
   rdfs:comment """In this form of DBMS connectivity, a driver uses its own networking functionality to connect to a
			3rd party DBMS. It has the advantage of providing innovations [as part of the driver] in critical
			areas such as privacy,security, and cost-effective adminsitration. """@en  ;
   rdfs:isDefinedBy <http://www.openlinksw.com/ontology/odbc#> .


# <-------------- ODBC Ontology Instances of Class --------------> #

odbc:PHP a oplsof:ApplicationProgram ;
   rdfs:label "PHP"@en  ;
   rdfs:seeAlso dbpedia:PHP ;
   rdfs:isDefinedBy <http://www.openlinksw.com/ontology/odbc#> .


# <-------------- ODBC Ontology Properties --------------> #

odbc:hasCursorSupport a rdf:Property , owl:ObjectProperty ;
   rdfs:label "hasScrollableCursorSupport"@en  ;
   skos:altLabel "Scrollable Cursor Support"@en  ;
   rdfs:comment """ODBC Drivers support of Scrollable Cursors. """@en  ;
   rdfs:domain odbc:OpenDatabaseConnectivityDriver ;
   rdfs:range odbc:ScrollableCursor ;
   rdfs:isDefinedBy <http://www.openlinksw.com/ontology/odbc#> .

odbc:isChangeSenstive a rdf:Property , owl:ObjectProperty ;
   rdfs:label "isChangeSenstive"@en  ;
   skos:altLabel "Is Change Sensitive"@en  ;
   rdfs:comment """Change sensitivity of an ODBC Drivers Scrollable Cursor implementation. """@en  ;
   rdfs:domain odbc:StaticScrollableCursor, odbc:KeySetScrollableCursor;
   rdfs:range xsd:boolean ;
   rdfs:isDefinedBy <http://www.openlinksw.com/ontology/odbc#> .

odbc:isFullyChangeSenstive a rdf:Property , owl:ObjectProperty ;
   rdfs:label "isFullyChangeSenstive"@en  ;
   skos:altLabel "Is Fully Change Sensitive"@en  ;
   rdfs:comment """Change sensitivity of an ODBC Drivers Scrollable Cursor implementation. """@en  ;
   rdfs:domain odbc:DynamicScrollableCursor;
   rdfs:range xsd:boolean ;
   rdfs:isDefinedBy <http://www.openlinksw.com/ontology/odbc#> .

odbc:isKeySetDriven a rdf:Property , owl:ObjectProperty ;
   rdfs:label "isKeySetDriven"@en  ;
   skos:altLabel "Keyset Driven"@en  ;
   rdfs:comment """Static Keyset based mechanism used to determine order and membership of an ODBC Driver's Scrollable Cursor implementation. """@en  ;
   rdfs:domain odbc:KeySetScrollableCursor ;
   rdfs:range xsd:boolean ;
   rdfs:isDefinedBy <http://www.openlinksw.com/ontology/odbc#> .

odbc:isDynamicKeySetDriven a rdf:Property , owl:ObjectProperty ;
   rdfs:label "isDynamicKeySetDriven"@en  ;
   skos:altLabel "Dynamic Keyset Driven"@en  ;
   rdfs:comment """Dynamic Keyset based mechanism used to determine order and membership of an ODBC Driver's Scrollable Cursor implementation. """@en  ;
   rdfs:domain odbc:MixedScrollableCursor;
   rdfs:range xsd:boolean ;
   rdfs:isDefinedBy <http://www.openlinksw.com/ontology/odbc#> .

odbc:hasConnectionPoolingSupport a rdf:Property , owl:ObjectProperty ;
   rdfs:label "hasConnectionPoolingSupport"@en  ;
   skos:altLabel "Connection Pooling Support"@en  ;
   rdfs:comment """ODBC Driver's ability to support pooled DBMX connnections that can be shared across many ODBC applications. """@en  ;
   rdfs:domain odbc:OpenDatabaseConnectivityDriver ;
   rdfs:range xsd:boolean ;
   rdfs:isDefinedBy <http://www.openlinksw.com/ontology/odbc#> .

odbc:hasRealApplicationClustorSupport a rdf:Property , owl:ObjectProperty ;
   rdfs:label "hasRealApplicationClustorSupport"@en  ;
   skos:altLabel "Real Application Cluster Support"@en  ;
   rdfs:comment """ODBC Driver's ability to support DBMS shared-nothing cluster configurations. """@en  ;
   rdfs:domain odbc:OpenDatabaseConnectivityDriver ;
   rdfs:range xsd:boolean ;
   rdfs:isDefinedBy <http://www.openlinksw.com/ontology/odbc#> .

odbc:hasMultipleActiveStatementsSupport a rdf:Property , owl:ObjectProperty ;
   rdfs:label "hasMultipleActiveStatementsSupport"@en  ;
   skos:altLabel "Multiple Active Statements Support"@en  ;
   rdfs:comment """ODBC Driver's ability to support multiple active statements on a single DBMS connection. This
				   capability is less resource intensive than opening up a new connection per statement. """@en  ;
   rdfs:domain odbc:OpenDatabaseConnectivityDriver ;
   rdfs:range xsd:boolean ;
   rdfs:isDefinedBy <http://www.openlinksw.com/ontology/odbc#> .

odbc:isOpsysArchitectureCompliant a rdf:Property , owl:ObjectProperty ;
   rdfs:label "isOpsysArchitectureCompliant"@en  ;
   skos:altLabel "Operating System Architecture Compliance"@en  ;
   rdfs:comment """Computer host operating system architecture supported e.g., 32-Bit, 64-Bit etc.. """@en  ;
   xhv:related dbpedia:64-bit_computing, dbpedia:32-bit_computing ;
   rdfs:domain odbc:OpenDatabaseConnectivityDriver ;
   rdfs:range oplsof:OperatingSystem ;
   rdfs:isDefinedBy <http://www.openlinksw.com/ontology/odbc#> .

odbc:isUsableWith a rdf:Property , owl:ObjectProperty ;
   rdfs:label "isUsableWith"@en  ;
   skos:altLabel "ODBC Application Compatibility"@en  ;
   rdfs:comment """ODBC Compliant Applications that driver works with, post-installation. Basically, applications that have been certified to work by driver vendor. """@en  ;
   rdfs:domain odbc:OpenDatabaseConnectivityDriver ;
   rdfs:range oplsof:ApplicationProgram ;
   rdfs:isDefinedBy <http://www.openlinksw.com/ontology/odbc#> .

odbc:hasOSAvailability a rdf:Property , owl:ObjectProperty ;
   rdfs:label "hasOSAvailability"@en  ;
   skos:altLabel "Supported Operating Systems"@en  ;
   owl:equivalentProperty oplsof:hasOperatingSystem  ;
   rdfs:comment """Operating Systems on which an ODBC Driver is available. """@en  ;
   rdfs:domain odbc:OpenDatabaseConnectivityDriver ;
   rdfs:range oplsof:OperatingSystem ;
   rdfs:isDefinedBy <http://www.openlinksw.com/ontology/odbc#> .

odbc:hasDBMSReleaseSupport a rdf:Property , owl:ObjectProperty ;
   rdfs:label "hasDBMSReleaseSupport"@en  ;
   owl:equivalentProperty oplsof:hasDatabaseEngine ;
   skos:altLabel "SQL RDBMS Release Support"@en  ;
   rdfs:comment """SQL Relational Database Management System Releases supported by an ODBC Driver. """@en  ;
   rdfs:domain odbc:OpenDatabaseConnectivityDriver ;
   rdfs:range oplsof:DbmsEngine ;
   rdfs:isDefinedBy <http://www.openlinksw.com/ontology/odbc#> .

odbc:isODBCLevelCompliant a rdf:Property , owl:DatatypeProperty ;
   rdfs:label "isODBCLevelCompliant"@en  ;
   skos:altLabel "ODBC Compliance Level"@en  ;
   rdfs:comment """ODBC Compliance levels supported by an ODBC Driver. """@en  ;
   rdfs:domain odbc:OpenDatabaseConnectivityDriver ;
   rdfs:range xsd:decimal ;
   rdfs:isDefinedBy <http://www.openlinksw.com/ontology/odbc#> .


odbc:hasScrollableCursorTypeSupport a rdf:Property , owl:ObjectProperty;
   rdfs:label "hasScrollableCursorTypeSupport"@en  ;
   skos:altLabel "Scrollable Cursor Type Support"@en  ;
   rdfs:comment """Types of Scrollable Cursors supported by an ODBC Driver. This feature
				determines the types of record paging and change-sensitivity combinations
				that a driver provides to ODBC compliant applications. """@en  ;
   xhv:related dbpedia:Scrollable_cursors ;
   rdfs:domain odbc:OpenDatabaseConnectivityDriver ;
   rdfs:range odbc:StaticScrollableCursor ;
   rdfs:isDefinedBy <http://www.openlinksw.com/ontology/odbc#> .

odbc:hasMultipleActiveStatementsSupport a rdf:Property , owl:ObjectProperty;
   rdfs:label "hasMultipleActiveStatementsSupport"@en  ;
   skos:altLabel "Supports Multiple Active Statements"@en  ;
   rdfs:comment """Multiple Active Statements supported by an ODBC Driver. """@en  ;
   xhv:related dbpedia:Distributed_transaction, dbpedia:Transaction_processing_system ;
   rdfs:domain odbc:OpenDatabaseConnectivityDriver ;
   rdfs:range odbc:DistributedTransactionMonitor ;
   rdfs:isDefinedBy <http://www.openlinksw.com/ontology/odbc#> .

odbc:hasDistributedTransactionMonitorSupport a rdf:Property , owl:ObjectProperty;
   rdfs:label "hasDistributedTransactionMonitorSupport"@en  ;
   skos:altLabel "Scrollable Cursor Type Support"@en  ;
   rdfs:comment """Distributed Transaction Monitors supported by an ODBC Driver. This feature
				determines the transaction monitor and associated distributed transaction functionality
				that a driver provides to ODBC compliant applications. """@en  ;
   xhv:related dbpedia:Distributed_transaction, dbpedia:Transaction_processing_system ;
   rdfs:domain odbc:OpenDatabaseConnectivityDriver ;
   rdfs:range odbc:DistributedTransactionMonitor ;
   rdfs:isDefinedBy <http://www.openlinksw.com/ontology/odbc#> .

odbc:hasDataTransmissionEncryptionSupport a rdf:Property , owl:DatatypeProperty ;
   rdfs:label "hasDataTransmissionEncryptionSupport"@en  ;
   skos:altLabel "Supports Encrypted Data Transmission"@en  ;
   rdfs:comment """Ability of an ODBC Driver to securely exchange data with an RDBMS using encryption. Ideally,
				this would be based on open standards such as Public Key Infrastructure (PKI) and Transport Layer Security (TLS). """@en  ;
   xhv:related dbpedia:Public_key_infrastructure, dbpedia:Transport_Layer_Security ;
   rdfs:domain odbc:OpenDatabaseConnectivityDriver ;
   rdfs:range xsd:boolean ;
   rdfs:isDefinedBy <http://www.openlinksw.com/ontology/odbc#> .

odbc:hasFineGrainedAccessControls a rdf:Property , owl:DatatypeProperty ;
   rdfs:label "hasFineGrainedAccessControls"@en  ;
   skos:altLabel "Supports Fine-grained Access Controls"@en  ;
   rdfs:comment """Ability of an ODBC Driver to provide controlled access to RDBMS server hosted data using
				fine-grained attribute based access controls scoped to identity principals. These controls
				as driven a combination of open standards associated with verifiable identity, identity authentication
				protocols, and rules for controlling query, create, update, insert, and delete operations. """@en  ;
   xhv:related dbpedia:Attribute-based_access_control, dbpedia:Public_key_infrastructure,
			dbpedia:Transport_Layer_Security ;
   rdfs:domain odbc:OpenDatabaseConnectivityDriver ;
   rdfs:range xsd:boolean ;
   rdfs:isDefinedBy <http://www.openlinksw.com/ontology/odbc#> .

odbc:hasDatabaseNetworkConnectivityMethod a rdf:Property , owl:ObjectProperty ;
   rdfs:label "hasDatabaseNetworkConnectivityMethod"@en  ;
   skos:altLabel "Database Connectivity Method over Network"@en  ;
   rdfs:comment """How an ODBC Driver connects to a target RDBMS. Fundamentally, this is achieved using
				one of the following methods: wire-protocol [native], RDBMS vendor provided client networking product [for use by 3rd parties],
				or RDBMS vendor independent networking built into a driver. """@en  ;
   xhv:related odbc:DBVendorNativeNetworkConnectivity, odbc:DBVendorProvidedNetworkConnectivity, odbc:DBVendorIndependentNetworkConnectivity ;
   xhv:related dbpedia:Public_key_infrastructure, dbpedia:Transport_Layer_Security ;
   rdfs:domain odbc:OpenDatabaseConnectivityDriver ;
   rdfs:range oplsof:DatabaseNetworkConnectivityMethod ;
   rdfs:isDefinedBy <http://www.openlinksw.com/ontology/odbc#> .

odbc:hasProtocolSupport a rdf:Property, owl:ObjectProperty ;
   rdfs:label "hasProtocolSupport" ;
   skos:altLabel "Has Protocol Support" ;
   rdfs:domain oplsof:DatabaseNetworkConnectivityMethod  ;
   rdfs:range oplsof:NetworkTransportProtocol ;
   rdfs:isDefinedBy <http://www.openlinksw.com/ontology/odbc#> .

